\documentclass{article}
\usepackage{amsthm}
\newtheorem*{proposition}{Proposition}

\begin{document}
	\Large
	\begin{proposition}
		S K K = I
	\end{proposition}
	\begin{proof}
		$S K K = (\lambda x \, y \, z. x \, z \, (y \, z)) \, (\lambda x \, y. x) \, (\lambda x \, y. x) 
		\\* \to_\alpha (\lambda a. \lambda b. \lambda z. a \, z \, (b \, z)) \, (\lambda x \, y. x) \, (\lambda x \, y. x)
		\\* \to_\beta (\lambda z. (\lambda x \, y. x) \, z \, ((\lambda x \, y. x) \, z))
		\\* \to_\beta (\lambda z. (\lambda y. z) \, (\lambda y. z))
		\\* \to_\beta (\lambda z. z) = I$
	\end{proof}
\end{document}
